implement `:-` without LHS, and
use PartiallyResolveTypeForMemberSelection to get Type instead of `?` in
error message

Source/Dafny/Printer.cs
@@ -1378,6 +1378,9 @@ namespace Microsoft.Dafny {
           PrintExpression(lhs, true);
           sep = ", ";
         }
+        if (s.Lhss.Count > 0) {
+          wr.Write(" ");
+        }
         PrintUpdateRHS(s, indent);
         wr.Write(";");
 
@@ -1406,6 +1409,7 @@ namespace Microsoft.Dafny {
           sep = ",";
         }
         if (s.Update != null) {
+          wr.Write(" ");
           PrintUpdateRHS(s.Update, indent);
         }
         wr.Write(";");
@@ -1473,14 +1477,15 @@ namespace Microsoft.Dafny {
     }
 
     /// <summary>
-    /// Does not print LHS
+    /// Does not print LHS, nor the space one might want between LHS and RHS,
+    /// because if there's no LHS, we don't want to start with a space
     /// </summary>
     void PrintUpdateRHS(ConcreteUpdateStatement s, int indent) {
       Contract.Requires(s != null);
       if (s is UpdateStmt) {
         var update = (UpdateStmt)s;
         if (update.Lhss.Count != 0) {
-          wr.Write(" := ");
+          wr.Write(":= ");
         }
         var sep = "";
         foreach (var rhs in update.Rhss) {
@@ -1490,14 +1495,14 @@ namespace Microsoft.Dafny {
         }
       } else if (s is AssignSuchThatStmt) {
         var update = (AssignSuchThatStmt)s;
-        wr.Write(" :| ");
+        wr.Write(":| ");
         if (update.AssumeToken != null) {
           wr.Write("assume ");
         }
         PrintExpression(update.Expr, true);
       } else if (s is AssignOrReturnStmt) {
         var stmt = (AssignOrReturnStmt)s;
-        wr.Write(" :- ");
+        wr.Write(":- ");
         PrintExpression(stmt.Rhs, true);
         if (DafnyOptions.O.DafnyPrintResolvedFile != null) {
           Contract.Assert(stmt.ResolvedStatements.Count > 0);  // filled in during resolution
